

1.  $e^{x-y}$

Maths

Let function  $f$  be  $f = e^{x-y}$

The first order partial derivatives of  $f$  is  $\frac{\partial f}{\partial x}$  &  $\frac{\partial f}{\partial y}$ .

$$\frac{\partial f}{\partial x} = \frac{\partial}{\partial x} (e^{x-y})$$

$$e^{x-y} \frac{\partial}{\partial x} (x-y)$$

$$e^{x-y} (1-0)$$

$$= e^{x-y}$$

$$\frac{\partial f}{\partial y} = \frac{\partial}{\partial y} (e^{x-y})$$

$$= e^{x-y} \frac{\partial}{\partial y} (x-y)$$

$$= e^{x-y} (0-1)$$

$$= -e^{x-y}$$

$\therefore$  The first order derivatives of  $e^{x-y}$  are  $\frac{\partial f}{\partial x} = e^{x-y}$ ,  $\frac{\partial f}{\partial y} = -e^{x-y}$

2. Euler's theorem on homogeneous function -

If  $z = f(x, y)$  is a homogeneous function of  $(x, y)$  of Degree 'n' then

$$x \frac{\partial z}{\partial x} + y \frac{\partial z}{\partial y} = n z \text{ for all } x, y \in \text{domain of the function.}$$

3. Neighbourhood of a point  $(a, b)$

Let  $\delta$  be any positive integer the points  $(x, y)$  such that  $a-\delta \leq x \leq a+\delta$

$$b-\delta \leq y \leq b+\delta.$$

Determined in a square bounded by the lines for  $x = a-\delta, a+\delta$ ;  $y = b-\delta, b+\delta$ . this square is called a neighbourhood of the point  $(a, b)$ .

$\therefore$  The set  $\{(x, y) : a-\delta \leq x \leq a+\delta, b-\delta \leq y \leq b+\delta\}$  is the neighbourhood of the point  $(a, b)$ .

# Section B

Question 1.

A.  $U = \log(x^2 + y^2 + z^2)$  prove that  $x \frac{\partial^2 U}{\partial y \partial x} = y \frac{\partial^2 U}{\partial x \partial y}$

sol Given  $U = \log(x^2 + y^2 + z^2)$

Then

$$\frac{\partial U}{\partial x} = \frac{\partial}{\partial x} (\log(x^2 + y^2 + z^2))$$

$$= \frac{1}{x^2 + y^2 + z^2} \frac{\partial}{\partial x} (x^2 + y^2 + z^2)$$

$$= \frac{1}{x^2 + y^2 + z^2} (2x + 0 + 0)$$

$$= \frac{2x}{x^2 + y^2 + z^2}$$

$$\frac{\partial U}{\partial y} = \frac{\partial}{\partial y} (\log(x^2 + y^2 + z^2))$$

$$= \frac{1}{x^2 + y^2 + z^2} \frac{\partial}{\partial y} (x^2 + y^2 + z^2)$$

$$= \frac{2y}{x^2 + y^2 + z^2}$$

$$\frac{\partial^2 U}{\partial y \partial x} = \frac{\partial}{\partial y} \left( \frac{\partial U}{\partial x} \right)$$

$$= \frac{\partial}{\partial y} \left( \frac{2x}{x^2 + y^2 + z^2} \right)$$

$$= 2x \left( \frac{-1}{(x^2 + y^2 + z^2)^2} \right) \frac{\partial}{\partial y} (x^2 + y^2 + z^2)$$

$$= \frac{-2x}{(x^2 + y^2 + z^2)^2} (2y + 0 + 0)$$

$$= \frac{-4xy}{(x^2 + y^2 + z^2)^2}$$

Mult  
Take  $x$  on both side

$$x \frac{\partial^2 U}{\partial y \partial x} = x \left( \frac{-4xy}{(x^2 + y^2 + z^2)^2} \right)$$

$$= \frac{-4x^2 y}{(x^2 + y^2 + z^2)^2} = \frac{-4xy}{(x^2 + y^2 + z^2)^2}$$

$$\frac{1}{x} = -\frac{1}{x^2}$$

$$\frac{\partial^2 U}{\partial x \partial y} = \frac{\partial}{\partial x} \left( \frac{\partial U}{\partial y} \right)$$

$$= \frac{\partial}{\partial x} \left( \frac{2y}{x^2 + y^2 + z^2} \right)$$

$$2y \left( \frac{-1}{(x^2 + y^2 + z^2)^2} \right) \frac{\partial}{\partial x} (x^2 + y^2 + z^2)$$

$$= \frac{-2y}{(x^2 + y^2 + z^2)^2} (2x + 0 + 0)$$

$$= \frac{-4xy}{(x^2 + y^2 + z^2)^2}$$

Mult  $y$  on both side

$$y \frac{\partial^2 U}{\partial x \partial y} = y \left( \frac{-4xy}{(x^2 + y^2 + z^2)^2} \right)$$

$$y \frac{\partial^2 U}{\partial x \partial y} = \frac{-4xy^2}{y(x^2 + y^2 + z^2)^2}$$



$$\therefore \frac{\partial^2 U}{\partial y \partial x} = \frac{\partial^2 U}{\partial x \partial y} \quad \text{Hence proved.}$$

B. Discuss Maxima & Minima of  $x^2 + xy$ .

Sol. Let the given function be  $f(x, y)$  then  $f = x^2 + xy$ .

Now will get values of  $\frac{\partial f}{\partial x}$  &  $\frac{\partial f}{\partial y}$ .

$$\begin{aligned} \frac{\partial f}{\partial x} &= \frac{\partial}{\partial x} (x^2 + xy) \\ &= 2x + (1)y \\ &= 2x + y. \end{aligned}$$

$$\begin{aligned} \frac{\partial f}{\partial y} &= \frac{\partial}{\partial y} (x^2 + xy) \\ &= 0 + x(1) \\ &= x. \end{aligned}$$

Now take  $\frac{\partial f}{\partial x} = 0$ ,

$$2x + y = 0 \rightarrow (1)$$

$$\frac{\partial f}{\partial y} = 0, \quad x = 0 \rightarrow (2)$$

substitute 2 in (1)

$$2(0) + y = 0$$

$$0 + y = 0 \therefore y = 0.$$

$\therefore (0, 0)$  is the stationary point.

$$\begin{aligned} \rightarrow r &= \frac{\partial^2 f}{\partial x^2} = \frac{\partial}{\partial x} \left( \frac{\partial f}{\partial x} \right) = \frac{\partial}{\partial x} (2x + y) \\ &= 2 + 0 = 2. \end{aligned}$$

$$s = \frac{\partial^2 f}{\partial y \partial x} = \frac{\partial}{\partial y} \left( \frac{\partial f}{\partial x} \right) = \frac{\partial}{\partial y} (2x + y) = 0 + 1 = 1.$$

$$t = \frac{\partial^2 f}{\partial y^2} = \frac{\partial}{\partial y} \left( \frac{\partial f}{\partial y} \right) = \frac{\partial}{\partial y} (x) = 0.$$

$$\begin{aligned} \text{then } rt - s^2 &= 2(0) - (1)^2 \\ &= 0 - 1 \\ &= -1 \end{aligned}$$

$rt - s^2 < 0, r > 0 \therefore f$  has no extreme values. At  $(0, 0)$

Question 2.

Verify Euler's theorem for  $z = x^n \log\left(\frac{y}{x}\right)$

Clearly  $z$  is a homogeneous function of degree  $n$  to verify Euler's theorem we have to prove that  $x \frac{\partial z}{\partial x} + y \frac{\partial z}{\partial y} = n z$ .

$$z = x^n (\log y - \log x)$$

Now,

$$\left[ \frac{\log m}{\log n} = \log m - \log n \right]$$

( $\therefore$  we apply uv here as there are  $\frac{\partial}{\partial x}$  in term).

$$\begin{aligned} \frac{\partial z}{\partial x} &= \frac{\partial}{\partial x} (x^n (\log y - \log x)) \\ &= x^n \frac{\partial}{\partial x} (\log y - \log x) + (\log y - \log x) \frac{\partial}{\partial x} (x^n) \\ &= x^n \left( 0 - \frac{1}{x} \right) + (\log y - \log x) n x^{n-1} \end{aligned}$$

$$\left[ n x^{n-1} = n \left( \frac{x^n}{x} \right) \right]$$

$$\begin{aligned} x \frac{\partial z}{\partial x} &= x \left( -\frac{x^n}{x} \right) + (\log y - \log x) (n x^n) \\ &= -x^n + (\log y - \log x) (n x^n) \end{aligned}$$

$$\begin{aligned} \frac{\partial z}{\partial y} &= \frac{\partial}{\partial y} (x^n (\log y - \log x)) \\ &= x^n \frac{\partial}{\partial y} (\log y - \log x) \\ &= x^n \left( \frac{1}{y} - 0 \right) \\ &= \frac{x^n}{y} \end{aligned}$$

$$y \frac{\partial z}{\partial y} = y \frac{x^n}{y} \quad y \frac{\partial z}{\partial y} = x^n$$

$$\begin{aligned} \therefore x \frac{\partial z}{\partial x} + y \frac{\partial z}{\partial y} &= -x^n + (\log y - \log x) (n x^n) + x^n \\ &= (\log y - \log x) (n x^n) \\ &= n x^n (\log y - \log x) \quad [\because x^n (\log y - \log x) = z] \\ &= n z \end{aligned}$$

Hence Euler's theorem is verified  
i.e.  $x \frac{\partial z}{\partial x} + y \frac{\partial z}{\partial y} = n z$ .



6 find  $\frac{dy}{dx}$  for  $x^3 + y^3 = 3axy$ .

Given  $x^3 + y^3 = 3axy$ ,  $x^3 + y^3 - 3axy = 0$ .

We know

let the given fn be  $f(x, y) = x^3 + y^3 - 3axy = 0$ :

$$\begin{aligned} \text{We know that } \frac{\partial F}{\partial x} &= \frac{\partial}{\partial x} (x^3 + y^3 - 3axy) \\ &= 3x^2 + 0 - 3ay \\ &= 3x^2 - 3ay \end{aligned}$$

$$\begin{aligned} \frac{\partial F}{\partial y} &= \frac{\partial}{\partial y} (x^3 + y^3 - 3axy) \\ &= 0 + 3y^2 - 3ax \\ &= 3y^2 - 3ax \end{aligned}$$

$\therefore$  we know that for fn  $f(x, y) = 0$ , then  $\frac{dy}{dx} = -\frac{f_x}{f_y}$ .

$$\begin{aligned} \frac{dy}{dx} &= -\frac{(3x^2 - 3ay)}{(3y^2 - 3ax)} = -\frac{3(x^2 - ay)}{3(y^2 - ax)} \\ &= -\frac{x^2 - ay}{y^2 - ax} = \frac{ay - x^2}{y^2 - ax} \end{aligned}$$

Question 3.

6  $u = x^2 - y^2$ ,  $x = 2s - 3t + 4$ ,  $y = -s + 8t - 5$ . find  $-\frac{\partial u}{\partial s}$ .

Sol. we know that  $\frac{\partial u}{\partial s} = \frac{\partial u}{\partial x} \frac{\partial x}{\partial s} + \frac{\partial u}{\partial y} \frac{\partial y}{\partial s}$ .

Given  $u = x^2 - y^2$ .

$$\frac{\partial u}{\partial x} = \frac{\partial}{\partial x} (x^2 - y^2) = 2x - 0 = 2x$$

$$\frac{\partial u}{\partial y} = \frac{\partial}{\partial y} (x^2 - y^2) = 0 - 2y = -2y$$

also  $x = 2s - 3t + 4$ .

$$\frac{\partial x}{\partial s} = \frac{\partial}{\partial s} (2s - 3t + 4) = 2(1) - 0 + 0 = 2$$

$$y = -s + 8t - 5$$

$$\frac{\partial y}{\partial s} = \frac{\partial}{\partial s} (-s + 8t - 5) = -1 + 0 - 0 = -1$$

$$Q1 \quad -\frac{\partial u}{\partial a} = (2x)(2) + (-2)(-1) = 4x + 2y.$$

Q2. a. & b.  $u = \log \left[ \frac{x^4 + y^4}{x + y} \right]$  show that  $x \frac{\partial u}{\partial x} + y \frac{\partial u}{\partial y} = 3$ .

sol Given  $u = \log \left[ \frac{x^4 + y^4}{x + y} \right]$

$$\begin{aligned} e^u &= \frac{x^4 + y^4}{x + y} = z \\ &= \frac{x^4 \left( 1 + \frac{y^4}{x^4} \right)}{x \left( 1 + \frac{y}{x} \right)} = x^3 \phi \left[ \frac{y}{x} \right]. \end{aligned}$$

By Euler's theorem we get.

$$x \frac{\partial u}{\partial x} + y \frac{\partial u}{\partial y} = 3.$$

$$\Rightarrow x \frac{\partial}{\partial x} (e^u) + y \frac{\partial}{\partial y} (e^u) = 3e^u$$

$$\Rightarrow x e^u \frac{\partial u}{\partial x} + y e^u \frac{\partial u}{\partial y} = 3e^u$$

$$e^u \left( x \frac{\partial u}{\partial x} + y \frac{\partial u}{\partial y} \right) = 3e^u$$

$$x \frac{\partial u}{\partial x} + y \frac{\partial u}{\partial y} = 3.$$

Hence proved.